STStoITree started proof

theories/STStoITree.v
@@ -55,20 +55,157 @@ f sm st1
         v <- trigger (Syscall fn args);;
         Vis (Choose {st': state | @step st0 (Some (event_sys fn args)) st' })
             (fun st1 => interpSTS step state_sort (proj1_sig st1))
-      end.
+      end
+  .
 
-        (* let (fn, args) := *)
-        (*     (iota _ (fun ev: event => exists st1, step st0 (Some ev) st1)) *)
-        (* in *)
-        (* v <- trigger (Syscall fn args);; *)
-        (* Vis (subevent _ (Choose {st': state | @step st0 None st' })) *)
-        (*     (fun st1 => interpSTS step state_sort (proj1_sig st1)) *)
+  Lemma observe_eta E R (itr0 itr1: itree E R)
+        (EQ: _observe itr0 = _observe itr1)
+    :
+      itr0 = itr1.
+  Proof.
+    erewrite (itree_eta_ itr0).
+    erewrite (itree_eta_ itr1).
+    f_equal. auto.
+  Qed.
+
+  Lemma interpSTS_red
+        (state: Type)
+        (step: state -> option event -> state -> Prop)
+        (state_sort: state -> sort)
+        (st0: state):
+    interpSTS step state_sort st0
+    =
+    match (state_sort st0) with
+    | angelic =>
+      Vis (Take {st': state | @step st0 None st' })
+          (fun st1 => interpSTS step state_sort (proj1_sig st1))
+    | demonic =>
+      Vis (Choose {st': state | @step st0 None st' })
+          (fun st1 => interpSTS step state_sort (proj1_sig st1))
+    | final z =>
+      Ret z↑
+    | vis =>
+      '(exist _ (event_sys fn args) _) <-
+      trigger (Choose {ev': event | exists st', @step st0 (Some ev') st' });;
+      v <- trigger (Syscall fn args);;
+      Vis (Choose {st': state | @step st0 (Some (event_sys fn args)) st' })
+          (fun st1 => interpSTS step state_sort (proj1_sig st1))
+    end
+  .
+  Proof.
+    eapply observe_eta. reflexivity.
+  Qed.
+
+  (* Set Primitive Projections.  *)
   
-  (* CoFixpoint interpSTS (state: Type) (step: state -> option event -> state -> Prop) : *)
-  (*   state -> itree Es Any.t := *)
-  (*   fun st0 => *)
-  (*     Vis (subevent _ (Choose {st': state | @step st0 None st' })) *)
-  (*         (fun st1 => interpSTS step (proj1_sig st1)). *)
+  (* Lemma interpSTS_final: *)
+  (*   forall state step state_sort (st1 : state) retv, *)
+  (*     (state_sort st1 = final retv) -> *)
+  (*     (interpSTS step state_sort st1) = Ret retv↑. *)
+  (* Proof. *)
+  (*   intros. erewrite interpSTS_red. rewrite H. reflexivity. *)
+  (* Qed. *)
 
 End CONV.
 
+Section INV.
+
+  Import ModSem.ModSem.
+  
+  Program Definition interpITree:
+    (itree eventE Any.t) -> semantics :=
+    fun itr =>
+      {|
+        STS.state := (itree eventE Any.t);
+        STS.step := step;
+        STS.initial_state := itr;
+        STS.state_sort := state_sort;
+      |}
+  .
+  Next Obligation. inv STEP; inv STEP0; ss. csc. rewrite SYSCALL in *. csc. Qed.
+  Next Obligation. inv STEP; ss. Qed.
+  Next Obligation. inv STEP; ss. Qed.
+
+End INV.
+
+Section PROOF.
+
+  Import Behavior.Beh.
+
+  Variable
+    (state: Type)
+    (step: state -> option event -> state -> Prop)
+    (state_sort: state -> sort).
+
+  Hypothesis wf_vis :
+    forall (st0 : state) (ev0 ev1 : option event) (st1 st2 : state),
+      state_sort st0 = vis ->
+      step st0 ev0 st1 -> step st0 ev1 st2 -> ev0 = ev1 /\ st1 = st2.
+
+  Hypothesis wf_angelic :
+    forall (st0 : state) (ev : option event) (st1 : state),
+      state_sort st0 = angelic -> step st0 ev st1 -> ev = None.
+
+  Hypothesis wf_demonic :
+    forall (st0 : state) (ev : option event) (st1 : state),
+      state_sort st0 = demonic -> step st0 ev st1 -> ev = None.
+  
+  Theorem beh_preserved:
+    forall (st0: state) (tr: Tr.t),
+      of_state
+        {|
+          STS.state := state;
+          STS.step := step;
+          STS.initial_state := st0;
+          STS.state_sort := state_sort;
+          STS.wf_vis := wf_vis;
+          STS.wf_angelic := wf_angelic;
+          STS.wf_demonic := wf_demonic;
+        |}
+        st0
+        tr
+      ->
+      of_state
+        (interpITree (interpSTS step state_sort st0))
+        (initial_state (interpITree (interpSTS step state_sort st0)))
+        tr.
+  Proof.
+    intros st0. pcofix CIH. i. punfold H0.
+    induction H0 using of_state_ind; ss; clarify.
+    - pfold. econs. ss.
+      erewrite interpSTS_red. rewrite H.
+      unfold ModSem.state_sort. ss.
+      (** type mismatch:
+          ModSem.state_sort assumes return type = val,
+          but
+          state of 'final' sort returns only Z. *)
+      admit "TODO: fix the return type".
+    - pfold. econs. clear CIH.
+      (* revert st1 H.  *)
+      pcofix CIH. punfold H. ss. inv H.
+      + pfold. econs 1.
+        * ss. erewrite interpSTS_red. rewrite SRT. ss.
+        * i. ss. rewrite interpSTS_red in STEP0. rewrite SRT in STEP0.
+          dependent destruction STEP0. destruct x as [st2 STEP0].
+          right. admit "paco bug".
+      + pfold. econs 2.
+          
+
+      
+
+    Abort.
+  (* paco gf r = gfp (fun x => r \/ gf (paco gf r)) *)
+   
+  (* Theorem beh_preserved: *)
+  (*   forall (sm: semantics) (st0: state sm) (tr: Tr.t), *)
+  (*     of_state *)
+  (*       sm *)
+  (*       st0 tr *)
+  (*     -> *)
+  (*     of_state *)
+  (*       (interpITree (interpSTS (step sm) (state_sort sm) st0)) *)
+  (*       st0 tr. *)
+                      
+
+
+End PROOF.
